

Vincent Breault (111 226 718)

### Question #3

Soit la récurrence suivante  $C(n) = \begin{cases} 0 & \text{si } n \leq 1 \\ 2C(\lfloor \frac{n}{3} \rfloor) + n & \text{si } n > 1 \end{cases}$

Supposons que  $n = 3^K$  (puissance de 3)

$$\begin{aligned} \text{Nous avons } C(3^K) &= 2 \cdot C(3^{K-1}) + 3^K \\ &= 2(2 \cdot C(3^{K-2}) + 3^{K-1}) + 3^K \\ &= 2(2(2 \cdot C(3^{K-3}) + 3^{K-2}) + 3^{K-1}) + 3^K \\ &= 8 \cdot C(3^{K-3}) + 3^K + 2 \cdot 3^{K-1} + 4 \cdot 3^{K-2} \end{aligned}$$

$$\langle \forall i \geq 0 \rangle \quad = 2^i \cdot C(3^{K-i}) + 2^0 3^K + 2^1 3^{K-1} + \dots + 2^{i-1} 3^{K-(i-1)}$$

$$\langle \text{avec } i=k \rangle \quad = 2^k \cdot C(3^0) + 2^0 3^K + 2^1 3^{K-1} + \dots + 2^{k-1} 3^{K-(k-1)}$$

$$= 0 + \sum_{j=0}^{k-1} 3^{K-j} 2^j$$

$$= \sum_{j=0}^{k-1} \frac{3^K}{3^j} 2^j$$

$$= 3^K \sum_{j=0}^{k-1} \left(\frac{2}{3}\right)^j$$

$$= 3^K \left( \frac{\left(\frac{2}{3}\right)^k - 1}{\frac{2}{3} - 1} \right)$$

$$= 3^K \left( \frac{\left(\frac{2}{3}\right)^k}{-\frac{1}{3}} - \frac{1}{-\frac{1}{3}} \right)$$

$$= 3^K \left( 3 - 3 \times \left(\frac{2}{3}\right)^k \right)$$

$$= 3^{K+1} - 3 \times 2^k$$

$$\begin{aligned}
 \langle \text{ave} \ k=\log_3 n \rangle &= 3^{\log_3 n + 1} - 3 \times 2^{\log_3 n} \\
 \langle \text{ave} \ 3^{\log_3 2} = 2 \rangle &= 3 \cdot n - 3 \times (3^{\log_3 2})^{\log_3 n} \\
 &= 3 \cdot n - 3 \times 3^{(\log_3 2)(\log_3 n)} \\
 &= 3 \cdot n - 3 \times (3^{\log_3 n})^{\log_3 2} \\
 &= 3 \cdot n - 3 \times n^{\log_3 2} \\
 &= 3 \cdot n - 3n^{0.6309}
 \end{aligned}$$